changed name of optConstFullT

Syntax.v
@@ -388,18 +388,18 @@ Definition MethodT (sig : Signature) := forall ty, ty (fst sig) -> ActionT ty (s
 Notation Void := (Bit 0).
 
 Notation Attribute A := (string * A)%type (only parsing).
-Section optConstFullT.
+Section RegInitValT.
   Variable x: FullKind.
-  Inductive optConstFullT :=
+  Inductive RegInitValT :=
   | Uninit
   | Init (c: ConstFullT x)
   | RegFileUninit num k (pf: x = SyntaxKind (Array num k))
   | RegFileInit num k (pf: x = SyntaxKind (Array num k)) (val: ConstT k)
   | RegFileHex num k (pf: x = SyntaxKind (Array num k)) (file: string)
   | RegFileBin num k (pf: x = SyntaxKind (Array num k)) (file: string).
-End optConstFullT.
+End RegInitValT.
 
-Definition RegInitT := Attribute (sigT optConstFullT).
+Definition RegInitT := Attribute (sigT RegInitValT).
 Definition DefMethT := Attribute (sigT MethodT).
 Definition RuleT := Attribute (Action Void).
 
@@ -436,29 +436,29 @@ Notation "l '[=]' r" :=
 Definition getRegFileRegisters m :=
   match m with
   | RegFile dataArray read write IdxNum Data init =>
-    (dataArray, existT optConstFullT (SyntaxKind (Array IdxNum Data))
+    (dataArray, existT RegInitValT (SyntaxKind (Array IdxNum Data))
                        match init with
                        | None => Uninit _
                        | Some init' => Init (SyntaxConst (ConstArray (fun _ => init')))
                        end) :: nil
   | RegFileFile dataArray read write IdxNum Data file _ =>
-    (dataArray, existT optConstFullT (SyntaxKind (Array IdxNum Data)) (Uninit _)) :: nil
+    (dataArray, existT RegInitValT (SyntaxKind (Array IdxNum Data)) (Uninit _)) :: nil
   | SyncRegFile isAddr dataArray read write IdxNum Data init =>
-    (dataArray, existT optConstFullT (SyntaxKind (Array IdxNum Data))
+    (dataArray, existT RegInitValT (SyntaxKind (Array IdxNum Data))
                        match init with
                        | None => Uninit _
                        | Some init' => Init (SyntaxConst (ConstArray (fun _ => init')))
                        end)
       ::
-      map (fun x => (snd x, existT optConstFullT (SyntaxKind Data)
+      map (fun x => (snd x, existT RegInitValT (SyntaxKind Data)
                                    match init with
                                    | None => Uninit _
                                    | Some init' => Init (SyntaxConst init')
                                    end)) read
   | SyncRegFileFile isAddr dataArray read write IdxNum Data file _ =>
-    (dataArray, existT optConstFullT (SyntaxKind (Array IdxNum Data)) (Uninit _))
+    (dataArray, existT RegInitValT (SyntaxKind (Array IdxNum Data)) (Uninit _))
       ::
-      map (fun x => (snd x, existT optConstFullT (SyntaxKind Data) (Uninit _))) read
+      map (fun x => (snd x, existT RegInitValT (SyntaxKind Data) (Uninit _))) read
   end.
 
 Definition getRegisters m :=
@@ -2596,15 +2596,15 @@ Definition makeModule (im : InModule) :=
 Definition makeConst k (c: ConstT k): ConstFullT (SyntaxKind k) := SyntaxConst c.
 
 Notation "'RegisterN' name : type <- init" :=
-  (MERegister (name%string, existT optConstFullT type (Init init)))
+  (MERegister (name%string, existT RegInitValT type (Init init)))
     (at level 12, name at level 99) : kami_scope.
 
 Notation "'Register' name : type <- init" :=
-  (MERegister (name%string, existT optConstFullT (SyntaxKind type) (Init (makeConst init))))
+  (MERegister (name%string, existT RegInitValT (SyntaxKind type) (Init (makeConst init))))
     (at level 12, name at level 99) : kami_scope.
 
 Notation "'RegisterU' name : type" :=
-  (MERegister (name%string, existT optConstFullT (SyntaxKind type) (Uninit _)))
+  (MERegister (name%string, existT RegInitValT (SyntaxKind type) (Uninit _)))
     (at level 12, name at level 99) : kami_scope.
 
 Section Positive.
@@ -2666,7 +2666,7 @@ Definition AddIndicesToNames name idxs := map (fun x => AddIndexToName name x) i
 Notation "'RegisterVec' name 'using' nums : type <- init" :=
   (MERegAry (
     map (fun idx =>
-      (AddIndexToName name idx, existT optConstFullT (SyntaxKind type) (Init (makeConst init)))
+      (AddIndexToName name idx, existT RegInitValT (SyntaxKind type) (Init (makeConst init)))
     ) nums
   ))
     (at level 12, name at level 9, nums at level 9) : kami_scope.
